<style>
    html {
        direction: rtl;
    }
    eqn, table, .katex {
        direction: ltr;
    }
</style>

$$\hat{r} = \cos{\theta}\hat{x} + \sin{\theta}\hat{y}$$
$$\hat{\theta} = -\sin{\theta}\hat{x} + \cos{\theta}\hat{y}$$
$$\hat{x} = \hat{r}\cos{\theta} - \sin{\theta}\hat{\theta}$$
$$\hat{y} = \hat{r}\sin{\theta} + \cos{\theta}\hat{\theta}$$
$$\overline{r} = |r|\hat{r}$$
$$\overline{v} = \dot{\overline{r}} = \dot{r}\hat{r} + r\dot{\theta}\hat{\theta}$$
$$\overline{a} = \ddot{\overline{r}} = (\ddot{r}-r\dot{\theta}^2)\hat{r} + (2\dot{r}\dot{\theta} + r\ddot{\theta})\hat{\theta}$$

1.
    1.
    $$r_{(t)} = kt^2 \rightarrow \dot{r_{(t)}} = \delta kt^{\delta -1} \rightarrow \ddot{r_{(t)}} = \delta ^{\delta - 1}kt^{\delta - 2}$$
    $$-r\dot{\theta} = -k\beta^2t^{\alpha}e^{2\beta/t}$$
    $$kt^2\dot{\theta}^2 = k\beta^2t^{\alpha}e^{2\beta/t}$$
    $$\dot{\theta} = \beta e^{\beta t}$$
    $$\theta = \frac{\beta e^{\beta t}}{\beta}$$
    $$\theta = e^{\beta t} + \frac{\pi}{2}$$
    $$\hat{r} = \cos{(e^{\beta t} + \frac{\pi}{2})}\hat{x} + \sin{(e^{\beta t} + \frac{\pi}{2})}\hat{y}$$
    $$|\overline{r}| = kt^{\alpha}$$
    $$\overline{r} = |\overline{r}|\hat{r}$$
    $$\Downarrow$$
    $$\overline{r} = kt^{\alpha}(\cos{(e^{\beta t} + \frac{\pi}{2})}\hat{x} + \sin{(e^{\beta t} + \frac{\pi}{2})}\hat{y})$$

    2.  

    $$(\overline{r}_A - \overline{r}_B)\hat{r} = (kt^{\alpha} - \frac{kt^{\alpha}}{2})\hat{r}$$
    $$(\overline{r}_A - \overline{r}_B)\hat{r} = \frac{kt^{\alpha}}{2}\hat{r}$$
    $$(\overline{r}_A - \overline{r}_B)\hat{r} = \frac{kt^{\alpha}}{2}\hat{r}$$

    $$v_A - v_B = \frac{kt^{\alpha - 1}}{2}\hat{r}$$

    3.

    $$\alpha = 2 \Rightarrow \frac{kt^{2}}{2}$$

2. .

    1.
    
    $$\dot{r}\hat{r} = u$$
    $$\dot{\theta}\hat{\theta} = \omega$$

    $$\dot{r}\hat{r} = u$$
    $$r\hat{r} = ut$$
    $$\ddot{r}\hat{r} = 0$$

    $$\dot{\theta}\hat{\theta} = \omega$$
    $$\theta\hat{\theta} = \omega t$$
    $$\ddot{\theta}\hat{\theta} = 0$$

    $$\overline{v} = \dot{\overline{r}} = u\hat{r} + ut\omega\hat{\theta}$$
    $$\overline{a} = -ut \omega^2\hat{r} + 2u\omega \hat{\theta}$$

    2.

    $$\overline{v} = u(\cos{\theta}\hat{x} + \sin{\theta}\hat{y}) + ut\omega(-\sin{\theta}\hat{x} + \cos{\theta}\hat{y})$$
    $$\overline{v} = (u\cos{\theta} - ut \omega \sin{\theta})\hat{x} + (u\sin{\theta} + ut \omega \cos{\theta})\hat{y}$$

    $$\overline{a} = (-ut\omega^2\cos{\theta} - 2u\omega\sin{\theta})\hat{x} + (-ut\omega^2 \sin{\theta} + 2ut\omega\cos{\theta})\hat{y}$$
3.
    נתון

    $$r_{(\theta)} = A_{(\theta)}$$
    $$\theta_{(t)} = \frac{\alpha t^2}{2}$$

    1.  
    
    $$[A] = M$$
    2.
    
    $$r_{(\theta)} = A_{(\theta)} \Rightarrow \dot{r}_{(\theta)} = \dot{A}_{(\theta)} \Rightarrow \ddot{r}_{(\theta)} = \ddot{A}_{(\theta)}$$
    $$\theta_{(t)} = \frac{\alpha t^2}{2} \Rightarrow \dot{\theta}_{(t)} = \alpha t \Rightarrow \ddot{\theta}_{(t)} = \alpha$$

    רכיב התאוצה הרדיאלי:  

    $$(\ddot{r} - r\dot{\theta}^2) = A\alpha - \frac{A\alpha t^2}{2}\alpha^2 t^2 = 0$$
    $$t = \pm \sqrt[]{\frac{2}{\alpha^2}}$$
    $$\Downarrow$$
    $$t = \sqrt[]{\frac{2}{\alpha^2}}$$
    $$\theta_{(t_0)} = \frac{\alpha}{2}\sqrt[]{\frac{2}{\alpha^2}}$$
    $$\theta_{(t_0)} = \frac{1}{\sqrt[]{2}}$$

    3.  

    $$\ddot{r} - r\dot{\theta}^2 = 2\dot{r}\dot{\theta} + r\ddot{\theta}$$
    $$\Downarrow$$
    $$A\alpha - \frac{A\alpha t^2}{2} = 2A\alpha t \alpha t + \frac{A \alpha t^2}{2}\alpha$$
    $$\frac{\alpha^2 }{2}t^4 + (\frac{5}{2}\alpha)t^2  - 1 = 0$$
    $$x = t^2$$
    $$\Downarrow$$
    $$\frac{\alpha^2 }{2}x^2 + (\frac{5}{2}\alpha)x  - 1 = 0$$
    $$x_{1,2} = \frac{-\frac{5}{2} \pm \sqrt[]{\frac{33}{4}}}{\alpha}$$
    $$\theta_1 = \frac{\alpha}{2}\frac{-\frac{5}{2}+\sqrt[]{\frac{33}{4}}}{\alpha}$$

4.
5.
6.
7.
תרשים כוחות על $m_1$  

$$F \rightarrow$$
$$N \leftarrow$$
$$\Downarrow$$
$$F-N=m_1a_1$$
תרשים כוחות על $m_2$  

$$N \rightarrow$$
$$\Downarrow$$
$$N=m_2a_2$$

$$\Downarrow$$
$$x_2 - x_1 = 0$$
$$\Downarrow$$
$$a_2 = a_1 = a$$
$$\Downarrow$$
$$m_1a_1 = m_1a$$
$$m_2a_2 = m_2a$$

שתי משוואות עם 2 נעלמים ($a, N$)  

$$a = \frac{N}{m_2}$$
$$F-N = \frac{m_1 N}{m_2}$$
$$N = \frac{Fm_2}{m_1 + m_2}$$
